Change DigitalSignatures.ec. Momentarily skip generic introduction of PRF in HtS and start on XMSS.

proofs/Cleanup/XMSS_TW.ec
@@ -1,17 +1,22 @@
 (* --- Require/Import --- *)
 (* -- Built-In (Standard Library) -- *)
-require import AllCore List Distr.
-
+require import AllCore List Distr FinType BitEncoding.
+require (*--*) ROM.
+(*---*) import BS2Int.
 
 (* -- Local -- *)
 require import FL_XMSS_TW.
-require (*--*) HashThenSign.
-
+require (*--*) DigitalSignatures KeyedHashFunctions HashThenSign.
+(*--*) import WOTS_TW.
 
 type mseed.
 type mkey.
 
-op mkg : mseed -> mkey.
+op mkg : mseed -> index -> mkey.
+
+op [lossless full uniform] dmseed : mseed distr.
+
+op [lossless full uniform] dmkey : mkey distr.
 
 (* Authentication paths in Fixed-Length XMSS-TW binary hash tree *)
 type apXMSSTW = apFLXMSSTW.
@@ -20,11 +25,151 @@ type apXMSSTW = apFLXMSSTW.
 type pkXMSSTW = pkFLXMSSTW.
 
 (* Secret keys *)
-type skXMSSTW = .
+type skXMSSTW = mseed * skFLXMSSTW.
 
 (* Messages *)
-type msgXMSSTW = msgWOTS.
+type msgXMSSTW.
 
 (* Signatures *)
-type sigXMSSTW = index * sigWOTS * apFLXMSSTW.
+type sigXMSSTW = mkey * sigFLXMSSTW.
 
+clone import FinType as MKey with
+  type t <= mkey.
+  
+clone import FinType as MsgXMSSTW with
+  type t <= msgXMSSTW.
+
+clone import FinProdType as MKeyMsgXMSSTW with
+  type t1 <- mkey,
+  type t2 <- msgXMSSTW,
+  theory FT1 <- MKey,
+  theory FT2 <- MsgXMSSTW
+  
+  proof *.
+
+
+clone import DigitalSignatures as SS with
+  type pk_t <- pkXMSSTW,
+  type sk_t <- skXMSSTW,
+  type msg_t <- msgXMSSTW,
+  type sig_t <- sigXMSSTW
+  
+  rename [theory] "KeyUpdating" as "XMSSTW"
+  
+  proof *.
+
+
+clone import ROM as MCORO with
+  type in_t <- mkey * msgXMSSTW,
+  type out_t <- msgFLXMSSTW,
+    op dout <- fun _ => dmsgFLXMSSTW,
+  type d_in_t <- int,
+  type d_out_t <- bool
+  
+  proof *.
+
+clone import MCORO.LazyEager as MCOROLE with
+  theory FinType <- MKeyMsgXMSSTW
+  
+  proof *. 
+
+module MCO = ERO.
+
+(* Signature queries *)
+op qS : { int | 0 <= qS <= l } as rng_qS.
+
+(* Random oracle (hash) queries *)
+op qH : { int | 0 <= qH } as ge0_qH. 
+
+print int2bs.
+
+clone import HashThenSign as HtS with
+  type pk_fl_t <- pkFLXMSSTW,
+  type sk_fl_t <- skFLXMSSTW,
+  type msg_fl_t <- msgFLXMSSTW,
+  type sig_fl_t <- sigFLXMSSTW,
+  type rco_t <- mkey,
+  type msg_al_t <- msgXMSSTW,
+    
+    op n <- l,
+    op qS <- qS,
+    op qH <- qH,
+    
+    op MSG_FL.enum <- map DigestBlock.insubd (map (int2bs (8 * n)) (range 0 (2 ^ (8 * n)))),
+    
+    op dmsg_fl <- dmsgFLXMSSTW,
+    op drco <- dmkey,
+
+  theory RCO <- MKey,
+  theory MSG_AL <- MsgXMSSTW,
+  theory MCORO <- MCORO,
+  theory MCOROLE <- MCOROLE
+
+  proof *.
+  realize ge0_n by smt(ge2_l).
+  realize rng_qS by exact: rng_qS.
+  realize ge0_qH by exact: ge0_qH.
+  realize dmsg_fl_ll by exact: dmsgFLXMSSTW_ll.
+  realize dmsg_fl_uni by exact: dmsgFLXMSSTW_uni.
+  realize dmsg_fl_fu by exact: dmsgFLXMSSTW_fu.
+  realize drco_ll by exact: dmkey_ll.
+  realize drco_uni by exact: dmkey_uni.
+  realize drco_fu by exact: dmkey_fu.
+  realize MSG_FL.enum_spec.
+    move=> m; rewrite count_uniq_mem 1:map_inj_in_uniq => [x y | |].
+    + rewrite ?mapP => -[i [/mem_range rng_i ->]] -[j [/mem_range rng_j ->]] eqins. 
+      rewrite -(DigestBlock.insubdK (int2bs (8 * n) i)) 1:size_int2bs; 1: smt(ge1_n).
+      rewrite -(DigestBlock.insubdK (int2bs (8 * n) j)) 1:size_int2bs; 1: smt(ge1_n). 
+      by rewrite eqins. 
+    + rewrite map_inj_in_uniq => [x y /mem_range rng_x /mem_range rng_y|].
+      rewrite -{2}(int2bsK (8 * n) x) 3:-{2}(int2bsK (8 * n) y) //; 1,2: smt(ge1_n).
+      by move=> ->. 
+    + by rewrite range_uniq.
+    rewrite -b2i1; congr; rewrite eqT mapP. 
+    exists (DigestBlock.val m).
+    rewrite DigestBlock.valKd mapP /=. 
+    exists (bs2int (DigestBlock.val m)).
+    rewrite mem_range bs2int_ge0 /= (: 8 * n = size (DigestBlock.val m)) 1:DigestBlock.valP //. 
+    by rewrite bs2intK bs2int_le2Xs.
+  qed.
+   
+(* Scheme *)
+module XMSS_TW : XMSSTW.Scheme = {
+  proc keygen() : pkXMSSTW * skXMSSTW  = {
+    var ms : mseed;
+    var pk : pkXMSSTW;
+    var skfl : skFLXMSSTW;
+    var sk : skXMSSTW;
+    
+    ms <$ dmseed;
+    
+    (pk, skfl) <@ FL_XMSS_TW.keygen();
+    
+    sk <- (ms, skfl);
+    
+    return (pk, sk);
+  }
+  
+  proc sign(sk : skXMSSTW, m : msgXMSSTW) : sigXMSSTW * skXMSSTW = {
+    var ms : mseed;
+    var skfl : skFLXMSSTW;
+    var idx : index;
+    var mk : mkey;
+    var cm : msgFLXMSSTW;
+    
+    ms <- sk.`1;
+    skfl <- sk.`2;
+    
+    idx <- skfl.`1;
+    
+    mk <- mkg ms idx;
+    
+    
+    
+    return witness;
+  }
+  
+  proc verify(pk : pkXMSSTW, m : msgXMSSTW, sig : sigXMSSTW) : bool = {
+    return witness;
+  }
+}.
